---
layout: post
title:  "4X03 - Lecture 12"
date:   2021-02-05 11:30:00 -0500
categories: 4X03
---

Interpolation: Newton's Formula
===

Ex: Say you get data every 15min, and you need to simulate the data
- You need interpolation to do this, to fill the gaps, how can you interpolate?
    - **Constant Interpolation**: Hold the last data value until the next data point
        - Not accurate, can run into problems in simulation
    - **Linear Interpolation**: Follow a line from one data point to the next
        - Better but still probably a little unrealistic
    - **Quadratic Interpolation**: Follow a curve from one data point to the next using a given equation
- What about with images, making a frame in between two frames?
    - Can just use linear interpolation, get a smoother transition of pixels, less bad in this scenario
- Interpolation also seen in things like Keras with upsampling, different possible settings

Interpolation: Newton's Formula
- We have done...
    1. Monomial (just solve system, very basic)
    2. Lagrange (good result, not good computationally)
- And now we'll do Newton
- The **basis functions** are of form:  
    $$\gamma_j (x) = (x - x_0)(x-x_1) ... (x-x_{j-1})$$
- The interpolation functions will be a combination of this. For example, for cubic:
    $$\gamma_0 (x) = 1$$
    $$\gamma_1 (x) = x-x_0$$  
    $$\gamma_2 (x) = (x-x_0)(x-x_1)$$
- The polynomial for this would then be:  
    $$P(x) = c_0 + c_1 (x-x_0) + c_2 (x-x_0)(x-x_1)$$  
    And here we would need to compute the constants
- Say we have polynomial of degree *n*:  
    $$P_n(x) = c_0 + c_1(x-x_0) + c_2(x-x_0)(x-x_1) + ... + c_n(x-x_0)(x-x_1) ... (x-x_{n-1})$$
    - We know that  
    $$P_n(x_0) = y_0$$  
    and all of the multiplications for $x_i - x_0$ would then be 0, meaning that  
    $$c_0 = y_0$$
    - If we move onto $x_1$,  
    $$P_n(x_1) = c_0 + c_1 (x_1 - x_0) = y_1$$  
    Again, the multiplications cancel out here, and this is what we're left with
    - For $x_2$,  
    $$P_n(x_2) = c_0 + c_1(x_2 - x_0) + c_2(x_2 - x_0)(x_2 - x_1)$$  
    At this point we already know $c_0$ and $c_1$, so we can easily find $c_2$
- We will be interpolating a function of $f(x_i, y_i)$, so we will denote the constants as $c_0 = f(x_0)$, and $y_i = f(x_i)$
    - From this notation, we get  
        $$c_0 = f(x_0)$$  
        $$c_1 = \frac{f(x_1) - f(x_0)}{x_1 - x_0} = f[x_0, x_1]$$  
        $$c_2 = \frac{f(x_2) - c_0 - c_1(x_2 - x_0)}{(x_2 - x_0)(x_2 - x_1)}$$  
        $$= \frac{f(x_2) - f(x_0) - \frac{f(x_1) - f(x_0)}{x_1 - x_0}}{(x_2 - x_0)(x_2 - x_1)}$$  
        With some work, we can show the above is the same as  
        $$= \frac{\frac{f(x_2) - f(x_1)}{x_2 - x_1} - \frac{f(x_1) - f(x_0)}{x_1 - x_0}}{x_2 - x_0}$$  
        Which can then be shown with divided difference notation  
        $$= \frac{f[x_1, x_2] - f[x_0, x_1]}{x_2 - x_1} = f[x_0, x_1, x_2]$$
- **Divided difference** are defined by subtracting the *y* values over subtracting the *x* values, so as we saw:  
    $$f[x_i, x_{i+1}] = \frac{f(x_i) - f(x_{i+1})}{x_i - x_{i+1}}$$
    - These can be recursively defined, as seen with the $c_2$ example:  
        $$f[x_i, x_{i+1}, x_j] = \frac{f[x_{i+1}, x_j] - f[x_i, x_{j-1}]}{x_j - x_i}$$ 
- We can define any coefficients as:
    $$c_n = f[x_0, x_1, ..., x_n] = \frac{f[x_1, ..., x_n] - f[x_0, ..., x_{n-1}]}{x_i - x_0}$$

Ex2: We are given data points for *i* from 0 to 2, with $x_i = [1, 2, 4]$, $f[x_i] = y_i = [1, 3, 3]$
- We can add a column to our data table with the divided difference of values, with them being  
    $$f[a,b] = [-, 2, 0]$$
    - Note, $[-]$ values are null because they cannot be computed for the divided difference
- We can then add another column for triple divided difference values, being  
    $$f[a,b,c] = [-, -, -2/3]$$
- We can now get all of our coefficients, with $c_0 = 1, c_1 = 2, c_2 = -2/3$, giving us a final polynomial of  
    $$P_2(x) = c_0 + c_1(x-x_0) + c_2(x-x_0)(x-x_1)$$  
    $$1 + 2(x-1) - 2/3(x-1)(x-2)$$
    - We can check our polynomial by subbing in known *x* values and seeing given *y* values
- How can we then extend this polynomial, say if we have new data with $[x_3, y_3] = [3, 5]$?
    - We would need to compute the new resulting $f[a,b]$, and $f[a,b,c]$, and the new new $f[a,b,c,d]$, giving us our new coefficient  
        ![img]({{ site.url }}/assets/4x03/bt.PNG)
- Main advantage would be ability to quickly add new points as new terms with new coefficients, rather than creating an entirely new function