---
layout: post
title:  "4AA4 - Approximation Rules"
date:   2020-11-30 12:30:00 -0400
categories: 4AA4
---

Three Rules to Approximate $D(z)$ from $D(s)$
- A direct comparison shows that given $D(s)$, the corresponding $D(z)$ can be obtained by substitution of an approximation for the frequency variable $s$:  
![img]({{ site.url }}/assets/4aa4/ar1.PNG)
- The specific substitutions can be seen below:  
![img]({{ site.url }}/assets/4aa4/ar2.PNG)

Summary of Discrete Equivalents
- Methods for analysis and design of continuous controls are well established
- Design a continuous control first, then carry out the desired stability, steady state, and transient analysis
- Then find a discrete equivalent to the continuous compensator
- A discrete compensator is to be implemented in a computer program, which requires that:
    - Different equations representing the continuous control must be approximated to algebraic equations, involving sums and products only
    - Several approximation techniques called Numerical Integration

How to go from $G(s)$ to $G(z)$?  
![img]({{ site.url }}/assets/4aa4/ar3.PNG)

Map from z-Plane to s-Plane
![img]({{ site.url }}/assets/4aa4/ar4.PNG)

View the Approximation from Another Angle
- In the z-transform, we have:  
$$z = e^{sT}$$  
- Consider the power series:  
$$e^x = 1 + x + \frac{x^2}{2!} + \frac{x^3}{3!} + ...$$
- Then, we consider the linear approximation as:  
$$z = e^{sT} = 1 + sT$$  
$$z = \frac{1}{e^{-sT}} = \frac{1}{1 - sT}$$  
$$z = \frac{e^{\frac{1}{2}sT}}{e^{-\frac{1}{2}sT}} = \frac{1 + sT/2}{1 - sT/2}$$

Stability Regions by Mapping Rules
- **Forward Rectangular Rule:**  
$$z \gets sT + 1$$  
![img]({{ site.url }}/assets/4aa4/ar5.PNG)
    - If the discrete system is stable, then the corresponding continuous system is stable under forward rectangular rule
    - It is possible that a continuous system is stable, but the corresponding discrete system is unstable
    - **Discrete Stable $\to$ Continuous Stable**
- **Backwards Rectangular Rule:**  
$$z \gets \frac{1}{1-Ts}$$  
![img]({{ site.url }}/assets/4aa4/ar6.PNG)
    - Consider the following:  
    $$z = \frac{1}{1-Ts} = \frac{1}{2} + (\frac{1}{1 - Ts} - \frac{1}{2}) = \frac12 + \frac12 + \frac{1+Ts}{1-Ts}$$
    - Hence, we write:  
    $$| z - \frac12 | = \frac12$$
    - It is possible the discrete system is stable, but the corresponding continuous is unstable
    - **Discrete Stable $\gets$ Continuous Stable**
- **Trapezoidal Rectangular Rule:**  
$$z \gets \frac{1+ Ts/2}{1 - Ts/2} \text{ (bilinear transformation)}$$  
![img]({{ site.url }}/assets/4aa4/ar7.PNG)
    - Under trapezoid rule, the stability region of the s-plane is mapped exactly to the stable region of the z-plane
    - **Continuous Stable $\leftrightarrow$ Discrete Stable**

Bilinear Transformation Maps Imaginary Axis in s-Plane to the Unit Circle in the z-Plane  
![img]({{ site.url }}/assets/4aa4/ar8.PNG)
- Proof: Having $s = j \Omega$, we have:  
$$\frac{1 + Ts/2}{1 - Ts/2} = \frac{1 + T(j\Omega)/2}{1 - T(j\Omega)/2}$$  
Hence,  
$$z \gets \frac{1 + j \omega}{1 - j \omega}, \text{ where } \omega = \frac{T}2\Omega$$  

Bilinear Transformation Maps the Inside of the Unit Circle in the z-Plane into the Left Half of the s-Plane
- By forcing $\omega = Ts/2$:  
![img]({{ site.url }}/assets/4aa4/ar9.PNG)

Revisit the Following System:  
$$D(s) = \frac{U(s)}{E(s)} = \frac{a}{s+a}$$  
- $u(t) = 1 - e^{-at}$
- By forward rule:  
$$u(kT) = (1 - aT) u (kT - T) + aTe(kT - T)$$    
![img]({{ site.url }}/assets/4aa4/ar10.PNG)  
Forward rectangular approximation is badly behaved for large $aT$ or $T/\tau$
- By backward rule:
$$(1 + aT)u(kT) = u(kT - T) + aTe(kT)$$  
![img]({{ site.url }}/assets/4aa4/ar11.PNG)  
Backward rectangular approximation is better behaved for large $aT$ or $T/\tau$ since discrete stable $\gets$ continuous stable

Final Value Theorem for Z-Transform
- The FVT for z-transforms states that if $\lim_{k \to \infty} x(k)$ exists, then:  
$$\lim_{k \to \infty} x(k) = \lim_{z \to 1}(z - 1)X(z)$$
- Example: step function $U(z) = \frac{z}{z-1}$, so that:  
$$\lim_{k \to \infty} u(k) = \lim_{z \to 1}(z-1)U(z) = \lim_{z \to 1}(z-1)\frac{z}{z-1}=\lim_{z\to 1} z = 1$$