---
layout: post
title:  "4AA4 - Closed Loop Discrete Systems"
date:   2020-11-16 12:30:00 -0400
categories: 4AA4
---

Transfer Function of ZoH example in slides!

Block Diagram Reduction
- Are these sampled-data systems the same?
![img]({{ site.url }}/assets/4aa4/clds1.PNG)
- For the first one, we have:  
$$C(z) = G_1(z) G_2(z)E(z)$$  
- For the second one, we have:  
$$C(z)= Z[G_1(s) G_2(s)] E(z)$$
- Recall the presence of the sampler:  
$$r^*(t) = r(0) \delta(t) + r(T) \delta(t-T) + r(2T) \delta(t-2T) + ...$$  
    - From this, we get:  
    $$R^*(s) = \sum_{n=0}^\infty r(nT) e^{-nTs}$$
    - Consider:  
    $$R(s) = \int_0^\infty r(t) e^{-st} dt$$
![img]({{ site.url }}/assets/4aa4/clds2.PNG)
- Example (AAA)

Model for the Open-Loop System
![img]({{ site.url }}/assets/4aa4/clds3.PNG)
- The output of the open-loop system is:  
$$C(z) = G(z) D(z) E(z)$$  
Then the $c(kT)$ can be obtained accordingly

Closed Loop Sample Data System
![img]({{ site.url }}/assets/4aa4/clds4.PNG)
- We have:  
$$C(s) = G(s) E^*(s), E(s) = R(s) - H(s) C(s)$$  
From this we get:  
$$E(s) = R(s) - G(s) H(s) E^* (s)$$  
Therefore:  
$$E(z) = R(z) - Z[G(s) H(s)] E(z)$$
- We can now lay out the following: 
$$E(z) = \frac{R(z)}{1+Z[G(s) H(s)]}, C(z) = G(z) E(z)$$  
Therefore:  
$$C(z) = \frac{G(z) R(z)}{1+Z[G(s) H(s)]}$$

Closed Loop Transfer Function using Digital Sensing Device
- If we move the switch, as seen here:  
![img]({{ site.url }}/assets/4aa4/clds5.PNG)  
Then we get the following system of equations:  
$$C(s) = G(s)[R(s) - H(s) C^* (s)] = G(s) R(s) - G(s) H(s) C^*(s)$$  
$$C(z)(1 + Z(G(s) H(s))) = Z[G(s) R(s)]$$  
Therefore:  
$$C(z) = \frac{Z[G(s) R(s)]}{(1 + Z(G(s) H(s)))}$$

Closed Loop Transfer Function using Digital Controller
- We will now use multiple switches, as seen here:  
![img]({{ site.url }}/assets/4aa4/clds6.PNG)  
giving us the following equations:  
$$C(s) = G_2(s) U^*(s)$$  
$$U(s) = G_1(s) E^*(s)$$  
$$E(s) = R(s) - G_2(s)$$
- Applying z-transform, we have:  
$$C(z) = G_2(z) U^*(z)$$  
$$U(z) = G_1(z) E^*(z)$$  
$$E(z) = R(z) - Z[G_2(s) H(s)] U^*(z)$$  
- From all these, we end up with:  
$$\frac{C(z)}{R(z)} = \frac{G_1(z) G_1(z)}{1 + G_1(z) Z(G_2(s) H(s))}$$

Time Response
- Consider a continuous system:  
![img]({{ site.url }}/assets/4aa4/clds7.PNG)  
The closed loop transfer function is:  
$$T_s = \frac{4}{s+6}$$  
Hence the unit step response is:  
$$c(t) = 0.667(1 - e^{-6t})$$
- By adding a sampler and a ZoH, we get:  
![img]({{ site.url }}/assets/4aa4/clds8.PNG)  
- We can express the system output as:  
$$T(z) = \frac{G(z)}{1 + G(z)}$$  
where...  
$$G(z) = Z[\frac{1 - e^{-Ts}}{s} * \frac{4}{s+2}] = \frac{z-1}{z} * Z[\frac{4}{s(s + 2)}]$$  
$$ = \frac{z-1}{z} * \frac{2(1-e^{-2T})z}{(z-1))z-e^{-2T}}$$
- If $T = 0.1s$,  
$$ G(z) = \frac{0.3625}{z-0.8187}$$  
Hence,  
$$T(z) = \frac{G(z)}{1 + G(z)} = \frac{0.3625}{z - 0.4562}$$
- Since $R(z) = z/(z-1)$, we have:  
$$C(z) = \frac{G(z)}{1 + G(z)} R(z)$$  
Hence,  
$$C(z) = \frac{0.3625}{z-0.4562} * \frac{z}{z-1} = \frac{0.667z}{z-1} - \frac{0.667z}{z-0.4562}$$  
- This also gives us:  
$$c(kT) = 0.667[1 - 0.4562^k]$$  
![img]({{ site.url }}/assets/4aa4/clds9.PNG)  

