---
layout: post
title:  "4AA4 - Lecture 24"
date:   2020-11-12 12:30:00 -0400
categories: 4AA4
---

Further z-Transform Work
===

Using Partial Fraction Expression Method to Solve Inverse Z-Transform of $E_1(z)$
- Need to know the sum of a geometric series:  
$$\frac{z}{z-a} = 1 + az^{-1} + a^2z^{-1} + a^3 z^{-3} + ...$$  
$$= \sum_{k=0}^{\infty} a^k z^{-k}$$  
    1. Write $E_1(z)$:  
    $$E_1(z) = \frac{0.5z}{(z-1)(z-0.6)} = \frac{1.25z}{z-1} - \frac{1.25z}{z-0.6}$$  
    2. Write $E_1(z)$ in power series, so:  
    $$E_1(z) = 1.25 [\sum_{k=0}^{\infty} z^{-k} - \sum_{k=0}^{\infty} 0.6^k z^{-k}]$$  
    $$= 1.25 \sum_{k=0}^{\infty} (1-0.6^k) z^{-k}$$  
    3. AAA (finish)
