---
layout: post
title:  "4X03 - Lecture 9"
date:   2021-01-29 11:30:00 -0500
categories: 4X03
---

LU Decomposition
===

LU Decomposition
- Let $Ax = b$, where $A = LU$
- $L$ is a matrix given as:
    $$L =
    \begin{bmatrix}
    1 & 0 & 0 & ... \\
    X & 1 &  0 & ... \\
    Y & Z & 1  & ...\\
    ... & ... & ... & ...
    \end{bmatrix}
    $$
- $U$ is an upper triangular matrix
- We can then manipulate the formulas as follows:
    $$Ax = b$$
    $$LU x = b, y = Ux$$
    $$Ly = b$$
    $$Ux = y$$
- To solve these, it will take:
    $$LU: O(n^3)$$
    $$Ly = b: O(n^2)$$
    $$Ux = y: O(n^2)$$
    $$Ax = b^{(i)}, i = 1, ..., m, m \leq n$$
    For *m* systems, it would be $O(n^3)$, totalling $O(m*n^3)$, which when $m=n$, would be $O(n^4)$
- Look into other ways to compute $Ax = b^{(i)}, i = 1, ..., m$:
    - Compute $A = LU$:  
        For $i = 1, ..., m$:
        Solve $Ly = b^{(i)} (O(n^2))$
        Solve $Ux = y (O(n^2))$
    - Overall, this would computationally be $O(n^3 + mn^2)$
- Ex: Take the following matrix:
    $$A =
    \begin{bmatrix}
    1 & -1 & 3 \\
    1 & 1 &  0 \\
    3 & -2 & 1 \\
    \end{bmatrix}
    $$
    - Multiply the first row by 1 and subtract it from row 2, and multiply it by 3 and subtract it from row 3
    - Can also get this calculation into a matrix, multiplying each multiplication by -1 and multiplying it by the base matrix:
        $$M_1 * A = A^*$$
        $$\begin{bmatrix}
        1 & 0 & 0 \\
        -1 & 1 &  0 \\
        -3 & 0 & 1 \\
        \end{bmatrix}
        *
        \begin{bmatrix}
        1 & -1 & 3 \\
        1 & 1 &  0 \\
        3 & -2 & 1 \\
        \end{bmatrix}
        =
        \begin{bmatrix}
        1 & -1 & 3 \\
        0 & 2 &  -3 \\
        0 & 1 & -8 \\
        \end{bmatrix}
        $$
    - For the second operation, multiplying the second row by 1/2 and subtracting it from the bottom, gives us:
        $$M_2 * M_1 A = M_2 M_1 A = U
        $$
        \begin{bmatrix}
        1 & 0 & 0 \\
        0 & 1 &  0 \\
        0 & -1/2 & 1 \\
        \end{bmatrix}
        *
        \begin{bmatrix}
        1 & -1 & 3 \\
        0 & 2 &  -3 \\
        0 & 1 & -8 \\
        \end{bmatrix}
        =
        \begin{bmatrix}
        1 & -1 & 3 \\
        0 & 1 &  -3 \\
        0 & 0 & -6.5 \\
        \end{bmatrix}
        $$
    - We also have the following equations:
        $$M_2 M_1 A = U$$
        $$M_1 A = M_2^{-1} U$$
        $$A = M_1^{-1} M_2^{-1} U$$
        - Inverses of *M* matrices essentially just flip the negative signs on the non-diagonal entries, and multiplying the inverse *M* matrices together gives you a bottom triangular matrix of the values
    - This all generalizes to:
        $$M_{n-1}...M_2M_1A = U$$
        $$A = M_1^{-1}M_2^{-1} ... M_{n-1}^{-1} U$$
        These inverse *M* matrices all multiply up to *L*, giving us the final equation
        $$A = LU$$
        Giving us **LU decomposition without pivoting**
- Matlab has a function `lu` to do this for us
    - For matrix `A`, the equation would be `[L,U] = lu(A)`
    - Will give different but because they choose a different pivot
- What if we want to swap two rows?
    - To do this, we would need to multiply by a **permutation matrix**
    - A permutation matrix is a diagonal identity matrix which will change the order of the rows, for example, a permutation matrix from bottom left to top right would swap the first and third rows
