---
layout: post
title:  "4E03 - Lecture 9"
date:   2020-09-28 16:30:00 -0400
categories: 4E03
---

Operational Analysis Continued
===

Utilization Law  
- $\frac{B_i(t)}{t} = \frac{C_i(t)}{t} * \frac{B_i(t)}{C_i(t)}$  
- $\rho_i(t) = X_i(t)S_i(t)$
    - Letting $t \rarr \inf$,  
    $\rho_i = X_iE[S_i]$
    - Helpful since if we have two values, we can get the third
Forced Flow Law
    - Suppose that $A_i(t) = C_i(t)$. Let $E[V_i]$ be the expected number of visits to node *i* per job. This required a reference node, which we will call node 0. By definition, $E[V_0] = 1$. So, we have  
    $\lim_{t \rarr \inf} \frac{C_i(t)}{t} = \lim_{t \rarr \inf} \frac{C_0(t)}{t} E[V_i]$  
    $E[V_i] = \lim_{t \rarr \inf} \frac{C_i(t)}{C_0(t)}$
    - **Define**: System throughput *X* measured through node 0. The throughput of node *i* is  
    $$X_i(t) = \frac{C_i(t)}{t} = \frac{C_i(t)}{C_0(t)} \frac{C_0(t)}{t}$$  
    Taking the limit as $t \rightarrow \inf$...  
    $$X_i = E[V_i]X$$  

Device Demands
- Utilization Law: $\rho_i = X_i E[S_i]$
- Forced Flow Law: $X_i = E[V_i]X$
    - Combining these two: $\rho_i = E[S_i]E[V_i]X$
- Define the average demand at node *i*: $E[D_i] = E[S_i]E[V_i]$
- Then,   
$$\rho_i = E[D_i]X$$
- The **demand** at node *i*, $E[D_i]$, is the expected processing time at node *i* summed over all visits of a job. We will see that the *bottleneck* is the device with the highest $E[D_i]$
Little's Law
- $E[N_i] = \lambda_i E[T_i]$
    - This relates the number of jobs in a queueing system, $E[N_i], the arrival rate to the queueing system, $\lambda_i$ and the mean response time, $E[T_i]$
- Outline of Derivation
    - In lecture slides, not very important  

Users/Clients
- We consider a model where there are *M* users (clients) who operate as follows:
    1. Each user thinks for a period of time that has mean $E[Z]$ time units (the *think time*)
    2. At the end of a think time, the user submits the job/request to a subsystem
    3. Once processing is complete at the subsystem (and returned to the user), the user begins another think time
General Response Time Law
- Consider a system with *M* users connected to a subsystem with *K* nodes. We are interested in the mean response time for the subsystem, $E[T]$. Inside the subsystem, the mean number of jobs $E[N]$ satisfies:  
- $E[N] = XE[T]$  
$= E[N_1] + E[N_2] + ... + E[N_K]$  
- $XE[T] = X_1E[T_1] + X_2E[T_2] + ... + X_KE[T_K]$  
- $E[T] = E[V_1]E[T_1] + E[T_2]E[V_2] + ... + E[V_K]E[T_K]$
- This all goes to the final result:  
$E[T] = \sum_{i=1}{K} E[V_i]E[T_i]

Interactive Response Time Law
- Consider the same system as for the general response time law
- The total mean cycle time of a client's job is $E[Z] + E[T]$
- So, in a given time period of length *t*, each client generates, on average,  
$$\frac{t}{E[Z] + E[T]}$$  
requests.
- The throughput is given by:  
$$X = \frac{M(t/(E[Z] + E[T]))}{t}$$  
$$= \frac{M}{E[Z] + E[T]}$$
- The end result is:  
$$E[T] = \frac{M}{X} - E[Z]$$